Arithmetization/ISigmaOne/Metamath/Term/Functions.lean
@@ -8,585 +8,345 @@ open FirstOrder FirstOrder.Arith
 
 variable {V : Type*} [Zero V] [One V] [Add V] [Mul V] [LT V] [V ⊧ₘ* 𝐈𝚺₁]
 
+section
+
 variable {L : Arith.Language V} {pL : LDef} [Arith.Language.Defined L pL]
 
+namespace TermSubst
 
-/-
+def blueprint (pL : LDef) : Language.TermRec.Blueprint pL 2 where
+  bvar := .mkSigma “y n z m w | !znthDef y w z” (by simp)
+  fvar := .mkSigma “y n x m w | !qqFvarDef y x” (by simp)
+  func := .mkSigma “y n k f v v' m w | !qqFuncDef y k f v'” (by simp)
+
+variable (L)
+
+def construction : Language.TermRec.Construction V L (blueprint pL) where
+  bvar (param _ z)        := znth (param 1) z
+  fvar (_     _ x)        := &̂x
+  func (_     _ k f _ v') := f̂unc k f v'
+  bvar_defined := by intro v; simp [blueprint]; rfl
+  fvar_defined := by intro v; simp [blueprint]
+  func_defined := by intro v; simp [blueprint]; rfl
+
+end TermSubst
+
 section termSubst
 
-namespace FormalizedTermSubst
+open TermSubst
 
 variable (L)
 
-def Phi (n m w : V) (C : Set V) (p : V) : Prop :=
-  L.Semiterm n (π₁ p) ∧ L.Semiterm m (π₂ p) ∧
-  ( (∃ z < n, π₁ p = ^#z ∧ ⟪z, π₂ p⟫ ∈ w) ∨
-    (∃ x, π₁ p = ^&x ∧ π₂ p = ^&x) ∨
-    (∃ k f v v', π₁ p = ^func k f v ∧ π₂ p = ^func k f v' ∧ ∀ i u u', ⟪i, u⟫ ∈ v → ⟪i, u'⟫ ∈ v' → ⟪u, u'⟫ ∈ C) )
+def Language.termSubst (n m w t : V) : V := (construction L).result ![m, w] n t
 
-private lemma phi_iff (n m w C p : V) :
-    Phi L n m w {x | x ∈ C} p ↔
-    ∃ t₁ ≤ p, ∃ t₂ ≤ p, p = ⟪t₁, t₂⟫ ∧ L.Semiterm n t₁ ∧ L.Semiterm m t₂ ∧
-    ( (∃ z < n, t₁ = ^#z ∧ ⟪z, t₂⟫ ∈ w) ∨
-      (∃ x < t₁, t₁ = ^&x ∧ t₂ = ^&x) ∨
-      (∃ k < t₁, ∃ f < t₁, ∃ v < t₁, ∃ v' < t₂, t₁ = ^func k f v ∧ t₂ = ^func k f v' ∧
-        (∀ i < v, ∀ u < v, ∀ u' < v', ⟪i, u⟫ ∈ v → ⟪i, u'⟫ ∈ v' → ⟪u, u'⟫ ∈ C)) ) := by
-  constructor
-  ·{intro ⟨hp₁, hp₂, h⟩
-    refine ⟨π₁ p, by simp, π₂ p, by simp, by simp, hp₁, hp₂, ?_⟩
-    rcases h with (⟨z, hz, h₁, h⟩ | ⟨x, h₁, h₂⟩ | ⟨k, f, v, v', h₁, h₂, h⟩)
-    · left; exact ⟨z, hz, h₁, h⟩
-    · right; left; exact ⟨x, by simp [h₁], h₁, h₂⟩
-    · right; right
-      exact ⟨k, by simp [h₁], f, by simp [h₁], v, by simp [h₁], v', by simp [h₂],
-        h₁, h₂, fun i _ u _ u' _ hi hi' ↦ h i u u' hi hi'⟩}
-  · rintro ⟨t₁, _, t₂, _, rfl, ht₁, ht₂, h⟩
-    refine ⟨by simpa using ht₁, by simpa using ht₂, ?_⟩
-    rcases h with (⟨z, hz, rfl, h⟩ | ⟨x, _, rfl, rfl⟩ | ⟨k, _, f, _, v, _, v', _, rfl, rfl, h⟩)
-    · left; exact ⟨z, hz, by simp [h]⟩
-    · right; left; exact ⟨x, by simp⟩
-    · right; right
-      exact ⟨k, f, v, v', by simp, by simp, fun i u u' hi hi' ↦
-        h i (lt_of_mem_dom hi) u (lt_of_mem_rng hi) u' (lt_of_mem_rng hi') hi hi'⟩
-
-def formulaAux : Semisentence ℒₒᵣ 7 := “t₁ t₂ p C n m w |
-  (∃ z < n, !qqBvarDef t₁ z ∧ z ~[w] t₂) ∨
-  (∃ x < t₁, !qqFvarDef t₁ x ∧ !qqFvarDef t₂ x) ∨
-  (∃ k < t₁, ∃ f < t₁, ∃ v < t₁, ∃ v' < t₂, !qqFuncDef t₁ k f v ∧ !qqFuncDef t₂ k f v' ∧
-  (∀ i < v, ∀ u < v, ∀ u' < v', i ~[v] u → i ~[v'] u' → u ~[C] u'))”
-
-def formula (pL : LDef) : Fixpoint.Blueprint 3 := ⟨.mkDelta
-  (.mkSigma
-    “p C n m w |
-      ∃ t₁ <⁺ p, ∃ t₂ <⁺ p, !pairDef p t₁ t₂ ∧ !pL.isSemitermDef.sigma n t₁ ∧ !pL.isSemitermDef.sigma m t₂ ∧
-      !formulaAux t₁ t₂ p C n m w”
-    (by simp [formulaAux]))
-  (.mkPi
-    “p C n m w |
-      ∃ t₁ <⁺ p, ∃ t₂ <⁺ p, !pairDef p t₁ t₂ ∧ !pL.isSemitermDef.pi n t₁ ∧ !pL.isSemitermDef.pi m t₂ ∧
-      !formulaAux t₁ t₂ p C n m w”
-    (by simp [formulaAux]))⟩
-
-def construction : Fixpoint.Construction V (formula pL) where
-  Φ := fun v ↦ Phi L (v 0) (v 1) (v 2)
-  defined := ⟨fun v ↦
-    by simp [formula, HSemiformula.val_sigma, eval_isSemitermDef L, (isSemiterm_defined L).proper.iff'],
-  fun v ↦ by simpa [formula, HSemiformula.val_sigma, eval_isSemitermDef L, formulaAux] using phi_iff _ _ _ _ _ _⟩
-  monotone := by
-    rintro C C' hC v p ⟨ht₁, ht₂, (h | h | ⟨k, f, v, v', h₁, h₂, h⟩)⟩
-    · exact ⟨ht₁, ht₂, Or.inl h⟩
-    · exact ⟨ht₁, ht₂, Or.inr <| Or.inl h⟩
-    · exact ⟨ht₁, ht₂, Or.inr <| Or.inr ⟨k, f, v, v', h₁, h₂, fun i u u' hi hi' ↦ hC (h i u u' hi hi')⟩⟩
-
-instance : (construction L).StrongFinite V where
-  strong_finite := by
-    rintro C v p ⟨ht₁, ht₂, (h | h | ⟨k, f, v, v', h₁, h₂, h⟩)⟩
-    · exact ⟨ht₁, ht₂, Or.inl h⟩
-    · exact ⟨ht₁, ht₂, Or.inr <| Or.inl h⟩
-    · exact ⟨ht₁, ht₂, Or.inr <| Or.inr ⟨k, f, v, v', h₁, h₂, fun i u u' hi hi' ↦ ⟨h i u u' hi hi', by
-      have : ⟪u, u'⟫ < ⟪π₁ p, π₂ p⟫ := pair_lt_pair (by simpa [h₁] using lt_qqFunc_of_mem hi) (by simpa [h₂] using lt_qqFunc_of_mem hi')
-      simpa using this⟩⟩⟩
-
-def Subst (n m w : V) : V → Prop := (construction L).Fixpoint ![n, m, w]
-
-def _root_.LO.FirstOrder.Arith.LDef.substDef (pL : LDef) : 𝚫₁-Semisentence 4 :=
-  (formula pL).fixpointDefΔ₁.rew <| Rew.substs ![#3, #0, #1, #2]
-
-lemma subst_defined : 𝚫₁-Relation₄ (Subst L) via pL.substDef :=
-  ⟨HSemiformula.ProperOn.rew (construction L).fixpoint_definedΔ₁.proper _,
-   by intro v; simp [LDef.substDef, (construction L).eval_fixpointDefΔ₁, Subst]⟩
-
-@[simp] lemma eval_substDef (v) :
-    Semiformula.Evalbm V v pL.substDef.val ↔ Subst L (v 0) (v 1) (v 2) (v 3) := (subst_defined L).df.iff v
-
-instance subst_definable : 𝚫₁-Relation₄ (Subst L) := Defined.to_definable _ (subst_defined L)
-
-@[simp, definability] instance subst_definable' (Γ) : (Γ, m + 1)-Relation₄ (Subst L) :=
-  .of_deltaOne (subst_definable L) _ _
+def Language.termSubstSeq (k n m w v : V) : V := (construction L).resultSeq ![m, w] k n v
 
 variable {L}
 
-lemma Subst.case_iff {n m w p : V} :
-    Subst L n m w p ↔
-    L.Semiterm n (π₁ p) ∧ L.Semiterm m (π₂ p) ∧
-    ( (∃ z < n, π₁ p = ^#z ∧ ⟪z, π₂ p⟫ ∈ w) ∨
-      (∃ x, π₁ p = ^&x ∧ π₂ p = ^&x) ∨
-      (∃ k f v v', π₁ p = ^func k f v ∧ π₂ p = ^func k f v' ∧ ∀ i u u', ⟪i, u⟫ ∈ v → ⟪i, u'⟫ ∈ v' → Subst L n m w ⟪u, u'⟫) ) :=
-  (construction L).case
+variable {n m w : V}
 
-alias ⟨Subst.case, Subst.mk⟩ := Subst.case_iff
+@[simp] lemma termSubst_bvar {z} (hz : z < n) :
+    L.termSubst n m w #̂z = znth w z := by simp [Language.termSubst, hz, construction]
 
-lemma Subst.semiterm₁ {n m w t t'} (h : Subst L n m w ⟪t, t'⟫) : L.Semiterm n t := by simpa using h.case.1
+@[simp] lemma termSubst_fvar (x) :
+    L.termSubst n m w &̂x = &̂x := by simp [Language.termSubst, construction]
 
-lemma Subst.semiterm₂ {n m w t t'} (h : Subst L n m w ⟪t, t'⟫) : L.Semiterm m t' := by simpa using h.case.2.1
-
-lemma Subst.bvar {n m w z u : V} (hz : z < n) (hu : L.Semiterm m u) (h : ⟪z, u⟫ ∈ w) :
-    Subst L n m w ⟪^#z, u⟫ := Subst.mk ⟨by simp [hz], by simpa using hu, Or.inl ⟨z, hz, by simpa using h⟩⟩
-
-lemma Subst.bvar_iff {n m w z u : V} :
-    Subst L n m w ⟪^#z, u⟫ ↔ z < n ∧ L.Semiterm m u ∧ ⟪z, u⟫ ∈ w :=
-  ⟨by intro h
-      rcases h.case with ⟨_, hu, (⟨z', hz', hzz', h⟩ | ⟨x, h, _⟩ | ⟨k, f, v, v', h, _⟩)⟩
-      · rcases (show z = z' from by simpa using hzz'); exact ⟨hz', by simpa using hu, by simpa using h⟩
-      · simp [qqBvar, qqFvar] at h
-      · simp [qqBvar, qqFunc] at h,
-   by rintro ⟨hz, Hu, h⟩; exact Subst.bvar hz Hu h⟩
-
-@[simp] lemma Subst.fvar {n m w x : V} :
-    Subst L n m w ⟪^&x, ^&x⟫ := Subst.mk ⟨by simp, by simp, Or.inr <| Or.inl ⟨x, by simp⟩⟩
-
-lemma Subst.fvar_iff {n m w x u : V} :
-    Subst L n m w ⟪^&x, u⟫ ↔ u = ^&x := by
-  constructor
-  · intro h
-    rcases h.case with ⟨_, _, (⟨_, _, h, _⟩ | ⟨x', hx', h⟩ | ⟨_, _, _, _, h, _⟩)⟩
-    · simp [qqBvar, qqFvar] at h
-    · rcases (show x = x' from by simpa using hx'); simpa using h
-    · simp [qqFvar, qqFunc] at h
-  · rintro rfl; simp
-
-lemma Subst.func {n m w k f v v' : V}
-    (hkf : L.Func k f)
-    (hv : L.TermSeq k n v)
-    (hv' : L.TermSeq k m v')
-    (H : ∀ i u u', ⟪i, u⟫ ∈ v → ⟪i, u'⟫ ∈ v' → Subst L n m w ⟪u, u'⟫) :
-    Subst L n m w ⟪^func k f v, ^func k f v'⟫ :=
-  Subst.mk ⟨
-    by rw [pi₁_pair]; exact Semiterm.func hkf hv,
-    by rw [pi₂_pair]; exact Semiterm.func hkf hv',
-    Or.inr <| Or.inr ⟨k, f, v, v', by simp, by simp, H⟩⟩
-
-lemma Subst.func' {n m w k f v u : V} (h : Subst L n m w ⟪^func k f v, u⟫) :
-    ∃ v', Seq v' ∧ k = lh v' ∧ (∀ i u u', ⟪i, u⟫ ∈ v → ⟪i, u'⟫ ∈ v' → Subst L n m w ⟪u, u'⟫) ∧ u = ^func k f v' := by
-  rcases h.case with ⟨_, hu, (⟨_, _, h, _⟩ | ⟨x, h, _⟩ | ⟨k', f', v', v'', h₁, h₂, hv⟩)⟩
-  · simp [qqFunc, qqBvar] at h
-  · simp [qqFunc, qqFvar] at h
-  · rcases (show k = k' ∧ f = f' ∧ v = v' by simpa [qqFunc] using h₁) with ⟨rfl, rfl, rfl⟩
-    rcases (show u = ^func k f v'' by simpa using h₂)
-    have : L.Func k f ∧ Seq v'' ∧ k = lh v'' ∧ ∀ i u, ⟪i, u⟫ ∈ v'' → L.Semiterm m u := by simpa [Semiterm.func_iff] using hu
-    rcases this with ⟨_, Sv'', hk'', _⟩
-    exact ⟨v'', Sv'', hk'', hv, rfl⟩
-
-variable {n m w} (TSw : L.TermSeq n m w)
-
-lemma Subst.rng_exists {t : V} (ht : L.Semiterm n t) : ∃ u, Subst L n m w ⟪t, u⟫ := by
-  apply Semiterm.induction 𝚺 ?_ ?_ ?_ ?_ t ht
-  · definability
-  · intro z hz
-    have : ∃ u, ⟪z, u⟫ ∈ w := TSw.seq.exists (show z < lh w by simpa [TSw.lh] using hz)
-    rcases this with ⟨u, hu⟩
-    exact ⟨u, Subst.bvar hz (TSw.prop z u hu) hu⟩
-  · intro x; exact ⟨^&x, by simp⟩
-  · rintro k f v hkf hv ih
-    have : ∃ v', Seq v' ∧ lh v' = lh v ∧ ∀ i u', ⟪i, u'⟫ ∈ v' → ∀ u, ⟪i, u⟫ ∈ v → Subst L n m w ⟪u, u'⟫ := by
-      have : ∀ i < lh v, ∃ u', ∀ u, ⟪i, u⟫ ∈ v → Subst L n m w ⟪u, u'⟫ := by
-        intro i hi
-        have : ∃ u, Subst L n m w ⟪hv.seq.nth hi, u⟫ := ih i (hv.seq.nth hi) (by simp)
-        rcases this with ⟨u', hu'⟩
-        exact ⟨u', fun u hiuv  ↦ by rcases hv.seq.nth_uniq hi hiuv; exact hu'⟩
-      exact sigmaOne_skolem_seq
-        (by have : 𝚺₁-Relation fun x y ↦ ∀ u < v, ⟪x, u⟫ ∈ v → Subst L n m w ⟪u, y⟫ := by definability
-            exact this.of_iff fun w ↦ ⟨fun h u _ ↦ h u, fun h u hv ↦ h u (lt_of_mem_rng hv) hv⟩)
-        this
-    rcases this with ⟨v', Sv', hvv', h⟩
-    exact ⟨^func k f v',
-      Subst.func hkf hv ⟨Sv', by simp [hvv', hv.lh],
-        (fun i u' hi ↦ by
-          have : i < lh v := by simpa [hvv'] using Sv'.lt_lh_of_mem hi
-          exact h i u' hi (hv.seq.nth this) (by simp) |>.semiterm₂)⟩
-        (fun i u u' hi hi' ↦ h i u' hi' u hi)⟩
-
-lemma Subst.rng_unique
-    {t u₁ u₂ : V} : Subst L n m w ⟪t, u₁⟫ → Subst L n m w ⟪t, u₂⟫ → u₁ = u₂ := by
-  revert u₁ u₂
-  suffices L.Semiterm n t → ∀ u₁ u₂, Subst L n m w ⟪t, u₁⟫ → Subst L n m w ⟪t, u₂⟫ → u₁ = u₂
-  by intro u₁ u₂ h₁ h₂; exact this h₁.semiterm₁ u₁ u₂ h₁ h₂
-  intro ht
-  apply Semiterm.induction 𝚷 ?_ ?_ ?_ ?_ t ht
-  · definability
-  · simp only [bvar_iff, and_imp]
-    intro z _ u₁ u₂ _ _ h₁ _ _ h₂
-    exact TSw.seq.isMapping.uniq h₁ h₂
-  · simp [Subst.fvar_iff]
-  · intro k f v _ hv ih u₁ u₂ h₁ h₂
-    rcases Subst.func' h₁ with ⟨v₁, Sv₁, hk₁, hvv₁, rfl⟩
-    rcases Subst.func' h₂ with ⟨v₂, Sv₂, hk₂, hvv₂, rfl⟩
-    have : v₁ = v₂ := Sv₁.lh_ext Sv₂ (by simp [←hk₁, ←hk₂]) (by
-      intro i x₁ x₂ hxv₁ hxv₂
-      have hi : i < lh v := by simpa [←hv.lh, hk₁] using Sv₁.lt_lh_of_mem hxv₁
-      exact ih i (hv.seq.nth hi) (by simp) _ _ (hvv₁ _ _ _ (hv.seq.nth_mem hi) hxv₁) (hvv₂ _ _ _ (hv.seq.nth_mem hi) hxv₂))
-    rw [this]
-
-lemma Subst.rng_exists_unique {t : V} (ht : L.Semiterm n t) : ∃! u, Subst L n m w ⟪t, u⟫ := by
-  rcases Subst.rng_exists TSw ht with ⟨u, hu⟩
-  exact ExistsUnique.intro u hu (fun u' hu' ↦ Subst.rng_unique TSw hu' hu)
-
-variable (L)
-
-lemma Subst.rng_exists_unique_total (n m w t : V) :
-    ∃! u, (L.TermSeq n m w ∧ L.Semiterm n t → Subst L n m w ⟪t, u⟫) ∧ (¬(L.TermSeq n m w ∧ L.Semiterm n t) → u = 0) := by
-  by_cases h : L.TermSeq n m w ∧ L.Semiterm n t
-  · simp [h]; exact Subst.rng_exists_unique h.1 h.2
-  · simp [h]
-
-end FormalizedTermSubst
-
-open FormalizedTermSubst
-
-variable (L)
-
-def Language.termSubst (n m w t : V) : V := Classical.choose! (Subst.rng_exists_unique_total L n m w t)
-
-variable {L}
-
-def Language.TermSeq.spec_of_semiterm {n m w t : V} (TSw : L.TermSeq n m w) (ht : L.Semiterm n t) : Subst L n m w ⟪t, L.termSubst n m w t⟫ :=
-  Classical.choose!_spec (Subst.rng_exists_unique_total L n m w t) |>.1 ⟨TSw, ht⟩
-
-def Language.TermSeq.substs_isterm {n m w t : V} (TSw : L.TermSeq n m w) (ht : L.Semiterm n t) :
-    L.Semiterm m (L.termSubst n m w t) := TSw.spec_of_semiterm ht |>.semiterm₂
-
-def termSubst_spec {n m w t : V} :
-    ¬(L.TermSeq n m w ∧ L.Semiterm n t) → L.termSubst n m w t = 0 :=
-  Classical.choose!_spec (Subst.rng_exists_unique_total L n m w t) |>.2
-
-variable {n m w : V} (TSw : L.TermSeq n m w)
-
-lemma Language.TermSeq.termSubst_eq_of {t} (ht : L.Semiterm n t) (h : Subst L n m w ⟪t, u⟫) : L.termSubst n m w t = u :=
-  (TSw.spec_of_semiterm ht).rng_unique TSw h
-
-lemma termSubst_bvar {z : V} (hz : z < n) (hu : ⟪z, u⟫ ∈ w) : L.termSubst n m w (^#z) = u :=
-  TSw.termSubst_eq_of (by simp [hz]) (Subst.bvar hz (TSw.prop z u hu) hu)
-
-@[simp] lemma termSubst_fvar (x : V) : L.termSubst n m w (^&x) = ^&x :=
-  TSw.termSubst_eq_of (by simp) (by simp)
-
-lemma termSubst_func {k f v v' : V} (hfk : L.Func k f)
-    (hv : L.TermSeq k n v)
-    (hv' : L.TermSeq k m v')
-    (H : ∀ i u u', ⟪i, u⟫ ∈ v → ⟪i, u'⟫ ∈ v' → L.termSubst n m w u = u') : L.termSubst n m w (^func k f v) = ^func k f v' :=
-  TSw.termSubst_eq_of (Semiterm.func hfk hv)
-    (Subst.func hfk hv hv' (fun i u u' hi hi' ↦ by
-      rcases H i u u' hi hi'; exact TSw.spec_of_semiterm (hv.prop i u hi)))
+@[simp] lemma termSubst_func {k f v} (hkf : L.Func k f) (hv : L.SemitermSeq k n v) :
+    L.termSubst n m w (f̂unc k f v) = f̂unc k f (L.termSubstSeq k n m w v) := by
+  simp [Language.termSubst, construction, hkf, hv]; rfl
 
 section
 
+def _root_.LO.FirstOrder.Arith.LDef.termSubstDef (pL : LDef) : 𝚺₁-Semisentence 5 := (blueprint pL).result.rew <| Rew.substs ![#0, #1, #4, #2, #3]
+
+def _root_.LO.FirstOrder.Arith.LDef.termSubstSeqDef (pL : LDef) : 𝚺₁-Semisentence 6 := (blueprint pL).resultSeq.rew <| Rew.substs ![#0, #1, #2, #5, #3, #4]
+
 variable (L)
 
-private lemma termSubst_graph (u n m w t : V) :
-    u = L.termSubst n m w t ↔
-    (L.TermSeq n m w ∧ L.Semiterm n t → ∃ p ≤ (t + u + 1)^2, p = ⟪t, u⟫ ∧ Subst L n m w p) ∧ (¬(L.TermSeq n m w ∧ L.Semiterm n t) → u = 0) :=
-  Iff.trans (Classical.choose!_eq_iff (Subst.rng_exists_unique_total L n m w t)) ⟨by
-    rintro ⟨hp, hn⟩
-    exact ⟨fun h ↦ ⟨⟪t, u⟫, by simp, rfl, hp h⟩, hn⟩, by
-    rintro ⟨hp, hn⟩
-    exact ⟨fun h ↦ by rcases hp h with ⟨_, _, rfl, h⟩; exact h, hn⟩⟩
+lemma termSubst_defined : Arith.DefinedFunction (fun v ↦ L.termSubst (v 0) (v 1) (v 2) (v 3)) pL.termSubstDef := by
+  intro v; simpa [LDef.termSubstDef, Language.termSubst] using (construction L).result_defined ![v 0, v 1, v 4, v 2, v 3]
 
-def _root_.LO.FirstOrder.Arith.LDef.termSubstDef (pL : LDef) : 𝚺₁-Semisentence 5 := .mkSigma
-  “u n m w t | (!pL.termSeqDef.pi n m w ∧ !pL.isSemitermDef.pi n t → ∃ p <⁺ (t + u + 1)², !pairDef p t u ∧ !pL.substDef.sigma n m w p) ∧
-    (¬(!pL.termSeqDef.sigma n m w ∧ !pL.isSemitermDef.sigma n t) → u = 0)” (by simp)
-
-lemma termSubst_defined : 𝚺₁-Function₄ L.termSubst via pL.termSubstDef := by
-  intro v
-  simp [LDef.termSubstDef, termSubst_graph, HSemiformula.val_sigma, eval_termSeq L,
-    eval_isSemitermDef L, (termSeq_defined L).proper.iff', (isSemiterm_defined L).proper.iff', eval_substDef L, -and_imp, -not_and]
-  apply iff_of_eq; congr; simp [imp_iff_not_or]; rfl
-
-@[simp] lemma termSubst_defined_iff (v : Fin 5 → V) :
+@[simp] lemma eval_termSubstDef (v : Fin 5 → V) :
     Semiformula.Evalbm (L := ℒₒᵣ) V v pL.termSubstDef ↔ v 0 = L.termSubst (v 1) (v 2) (v 3) (v 4) := (termSubst_defined L).df.iff v
 
-instance termSubst_definable : 𝚺₁-Function₄ L.termSubst :=
+instance termSubst_definable : Arith.DefinableFunction ℒₒᵣ 𝚺₁ (fun v : Fin 4 → V ↦ L.termSubst (v 0) (v 1) (v 2) (v 3)) :=
   Defined.to_definable _ (termSubst_defined L)
-/-
-@[simp, definability] instance termSubst_definable' (Γ m) : (Γ, m + 1)-Function₄ L.termSubst :=
-  .of_sigmaOne (termSubst_definable L) _ _
--/
-instance termSubst_definable₂ (n m) : 𝚺₁-Function₂ (L.termSubst n m) := by
+
+instance termSubst_definable₂ (n m : V) : 𝚺₁-Function₂ (L.termSubst n m) := by
   simpa using DefinableFunction.retractiont (n := 2) (termSubst_definable L) ![&n, &m, #0, #1]
 
-@[simp, definability] instance termSubst_definable₂' (Γ l n m) : (Γ, l + 1)-Function₂ (L.termSubst n m) :=
+@[simp, definability] instance termSubst_definable₂' (Γ k) (n m : V) : (Γ, k + 1)-Function₂ (L.termSubst n m) :=
   .of_sigmaOne (termSubst_definable₂ L n m) _ _
+
+lemma termSubstSeq_defined : Arith.DefinedFunction (fun v ↦ L.termSubstSeq (v 0) (v 1) (v 2) (v 3) (v 4)) pL.termSubstSeqDef := by
+  intro v; simpa [LDef.termSubstSeqDef, Language.termSubstSeq] using (construction L).resultSeq_defined ![v 0, v 1, v 2, v 5, v 3, v 4]
+
+@[simp] lemma eval_termSubstSeqDef (v : Fin 6 → V) :
+    Semiformula.Evalbm (L := ℒₒᵣ) V v pL.termSubstSeqDef ↔ v 0 = L.termSubstSeq (v 1) (v 2) (v 3) (v 4) (v 5) := (termSubstSeq_defined L).df.iff v
+
+instance termSubstSeq_definable : Arith.DefinableFunction ℒₒᵣ 𝚺₁ (fun v : Fin 5 → V ↦ L.termSubstSeq (v 0) (v 1) (v 2) (v 3) (v 4)) :=
+  Defined.to_definable _ (termSubstSeq_defined L)
+
+instance termSubstSeq_definable₂ (k n m : V) : 𝚺₁-Function₂ (L.termSubstSeq k n m) := by
+  simpa using DefinableFunction.retractiont (n := 2) (termSubstSeq_definable L) ![&k, &n, &m, #0, #1]
+
+@[simp, definability] instance termSubstSeq_definable₂' (Γ i) (k n m : V) : (Γ, i + 1)-Function₂ (L.termSubstSeq k n m) :=
+  .of_sigmaOne (termSubstSeq_definable₂ L k n m) _ _
 
 end
 
+lemma termSubst_rng_semiterm {t} (hw : L.SemitermSeq n m w) (ht : L.Semiterm n t) : L.Semiterm m (L.termSubst n m w t) := by
+  apply Language.Semiterm.induction 𝚺 ?_ ?_ ?_ ?_ t ht
+  · definability
+  · intro z hz; simp [hz, hw.prop_znth]
+  · intro x; simp
+  · intro k f v hkf hv ih;
+    simp only [hkf, hv, termSubst_func, Language.Semiterm.func_iff, true_and]
+    exact ⟨by simp [Language.termSubstSeq, hv], by simp [Language.termSubstSeq, hv], fun i z hiz ↦ by
+      rcases (construction L).resultSeq_prop' _ hv hiz with ⟨u, hiu, rfl⟩
+      exact ih _ _ hiu⟩
+
+lemma termSubstSeq_rng_termSeq {k n m v} (hw : L.SemitermSeq n m w) (hv : L.SemitermSeq k n v) : L.SemitermSeq k m (L.termSubstSeq k n m w v) :=
+  ⟨by simp [Language.termSubstSeq, hv], by simp [Language.termSubstSeq, hv], fun i u hiu ↦ by
+    rcases (construction L).resultSeq_prop' _ hv hiu with ⟨u', hiu', rfl⟩
+    exact termSubst_rng_semiterm hw (hv.prop _ _ hiu')⟩
+
 end termSubst
+
+namespace TermShift
+
+def blueprint (pL : LDef) : Language.TermRec.Blueprint pL 0 where
+  bvar := .mkSigma “y n z m w | !qqBvarDef y z” (by simp)
+  fvar := .mkSigma “y n x m w | !qqFvarDef y (x + 1)” (by simp)
+  func := .mkSigma “y n k f v v' m w | !qqFuncDef y k f v'” (by simp)
+
+variable (L)
+
+def construction : Language.TermRec.Construction V L (blueprint pL) where
+  bvar (_ _ z)        := #̂z
+  fvar (_ _ x)        := &̂(x + 1)
+  func (_ _ k f _ v') := f̂unc k f v'
+  bvar_defined := by intro v; simp [blueprint]
+  fvar_defined := by intro v; simp [blueprint]
+  func_defined := by intro v; simp [blueprint]; rfl
+
+end TermShift
 
 section termShift
 
-namespace FormalizedTermShift
+open TermShift
 
 variable (L)
 
-def Phi (n : V) (C : Set V) (p : V) : Prop :=
-  L.Semiterm n (π₁ p) ∧ L.Semiterm n (π₂ p) ∧
-  ( (∃ z < n, π₁ p = ^#z ∧ π₂ p = ^#z) ∨
-    (∃ x, π₁ p = ^&x ∧ π₂ p = ^&(x + 1)) ∨
-    (∃ k f v v', π₁ p = ^func k f v ∧ π₂ p = ^func k f v' ∧ ∀ i u u', ⟪i, u⟫ ∈ v → ⟪i, u'⟫ ∈ v' → ⟪u, u'⟫ ∈ C) )
+def Language.termShift (n t : V) : V := (construction L).result ![] n t
 
-private lemma phi_iff (n C p : V) :
-    Phi L n {x | x ∈ C} p ↔
-    ∃ t₁ ≤ p, ∃ t₂ ≤ p, p = ⟪t₁, t₂⟫ ∧ L.Semiterm n t₁ ∧ L.Semiterm n t₂ ∧
-    ( (∃ z < n, t₁ = ^#z ∧ t₂ = ^#z) ∨
-      (∃ x < t₁, t₁ = ^&x ∧ t₂ = ^&(x + 1)) ∨
-      (∃ k < t₁, ∃ f < t₁, ∃ v < t₁, ∃ v' < t₂, t₁ = ^func k f v ∧ t₂ = ^func k f v' ∧
-        (∀ i < v, ∀ u < v, ∀ u' < v', ⟪i, u⟫ ∈ v → ⟪i, u'⟫ ∈ v' → ⟪u, u'⟫ ∈ C)) ) := by
-  constructor
-  ·{intro ⟨hp₁, hp₂, h⟩
-    refine ⟨π₁ p, by simp, π₂ p, by simp, by simp, hp₁, hp₂, ?_⟩
-    rcases h with (⟨z, hz, h₁, h⟩ | ⟨x, h₁, h₂⟩ | ⟨k, f, v, v', h₁, h₂, h⟩)
-    · left; exact ⟨z, hz, h₁, h⟩
-    · right; left; exact ⟨x, by simp [h₁], h₁, h₂⟩
-    · right; right
-      exact ⟨k, by simp [h₁], f, by simp [h₁], v, by simp [h₁], v', by simp [h₂],
-        h₁, h₂, fun i _ u _ u' _ hi hi' ↦ h i u u' hi hi'⟩}
-  · rintro ⟨t₁, _, t₂, _, rfl, ht₁, ht₂, h⟩
-    refine ⟨by simpa using ht₁, by simpa using ht₂, ?_⟩
-    rcases h with (⟨z, hz, rfl, h⟩ | ⟨x, _, rfl, rfl⟩ | ⟨k, _, f, _, v, _, v', _, rfl, rfl, h⟩)
-    · left; exact ⟨z, hz, by simp [h]⟩
-    · right; left; exact ⟨x, by simp⟩
-    · right; right
-      exact ⟨k, f, v, v', by simp, by simp, fun i u u' hi hi' ↦
-        h i (lt_of_mem_dom hi) u (lt_of_mem_rng hi) u' (lt_of_mem_rng hi') hi hi'⟩
-
-def formulaAux : Semisentence ℒₒᵣ 5 := “t₁ t₂ p C n |
-  (∃ z < n, !qqBvarDef t₁ z ∧ !qqBvarDef t₂ z) ∨
-  (∃ x < t₁, !qqFvarDef t₁ x ∧ !qqFvarDef t₂ (x + 1)) ∨
-  (∃ k < t₁, ∃ f < t₁, ∃ v < t₁, ∃ v' < t₂, !qqFuncDef t₁ k f v ∧ !qqFuncDef t₂ k f v' ∧
-  (∀ i < v, ∀ u < v, ∀ u' < v', i ~[v] u → i ~[v'] u' → u ~[C] u'))”
-
-def formula (pL : LDef) : Fixpoint.Blueprint 1 := ⟨.mkDelta
-  (.mkSigma
-    “p C n |
-      ∃ t₁ <⁺ p, ∃ t₂ <⁺ p, !pairDef p t₁ t₂ ∧ !pL.isSemitermDef.sigma n t₁ ∧ !pL.isSemitermDef.sigma n t₂ ∧
-      !formulaAux t₁ t₂ p C n”
-    (by simp [formulaAux]))
-  (.mkPi
-    “p C n |
-      ∃ t₁ <⁺ p, ∃ t₂ <⁺ p, !pairDef p t₁ t₂ ∧ !pL.isSemitermDef.pi n t₁ ∧ !pL.isSemitermDef.pi n t₂ ∧
-      !formulaAux t₁ t₂ p C n”
-    (by simp [formulaAux]))⟩
-
-def construction : Fixpoint.Construction V (formula pL) where
-  Φ := fun v ↦ Phi L (v 0)
-  defined := ⟨fun v ↦
-    by simp [formula, HSemiformula.val_sigma, eval_isSemitermDef L, (isSemiterm_defined L).proper.iff'],
-  fun v ↦ by simpa [formula, HSemiformula.val_sigma, eval_isSemitermDef L, formulaAux] using phi_iff _ _ _ _⟩
-  monotone := by
-    rintro C C' hC v p ⟨ht₁, ht₂, (h | h | ⟨k, f, v, v', h₁, h₂, h⟩)⟩
-    · exact ⟨ht₁, ht₂, Or.inl h⟩
-    · exact ⟨ht₁, ht₂, Or.inr <| Or.inl h⟩
-    · exact ⟨ht₁, ht₂, Or.inr <| Or.inr ⟨k, f, v, v', h₁, h₂, fun i u u' hi hi' ↦ hC (h i u u' hi hi')⟩⟩
-
-instance : (construction L).StrongFinite V where
-  strong_finite := by
-    rintro C v p ⟨ht₁, ht₂, (h | h | ⟨k, f, v, v', h₁, h₂, h⟩)⟩
-    · exact ⟨ht₁, ht₂, Or.inl h⟩
-    · exact ⟨ht₁, ht₂, Or.inr <| Or.inl h⟩
-    · exact ⟨ht₁, ht₂, Or.inr <| Or.inr ⟨k, f, v, v', h₁, h₂, fun i u u' hi hi' ↦ ⟨h i u u' hi hi', by
-      have : ⟪u, u'⟫ < ⟪π₁ p, π₂ p⟫ := pair_lt_pair (by simpa [h₁] using lt_qqFunc_of_mem hi) (by simpa [h₂] using lt_qqFunc_of_mem hi')
-      simpa using this⟩⟩⟩
-
-def Shift (n : V) : V → Prop := (construction L).Fixpoint ![n]
-
-def shiftDef (pL : LDef) : 𝚫₁-Semisentence 2 := (formula pL).fixpointDefΔ₁.rew <| Rew.substs ![#1, #0]
-
-lemma shift_defined : 𝚫₁-Relation (Shift L) via (shiftDef pL) :=
-  ⟨HSemiformula.ProperOn.rew (construction L).fixpoint_definedΔ₁.proper _,
-   by intro v; simp [shiftDef, (construction L).eval_fixpointDefΔ₁, Shift]⟩
-
-@[simp] lemma eval_shiftDef (v) :
-    Semiformula.Evalbm V v (shiftDef pL).val ↔ Shift L (v 0) (v 1) := (shift_defined L).df.iff v
-
-instance shift_definable : 𝚫₁-Relation (Shift L) := Defined.to_definable _ (shift_defined L)
-
-@[simp, definability] instance shift_definable' (Γ) : (Γ, m + 1)-Relation (Shift L) :=
-  .of_deltaOne (shift_definable L) _ _
+def Language.termShiftSeq (k n v : V) : V := (construction L).resultSeq ![] k n v
 
 variable {L}
-
-lemma Shift.case_iff {n p : V} :
-    Shift L n p ↔
-    L.Semiterm n (π₁ p) ∧ L.Semiterm n (π₂ p) ∧
-    ( (∃ z < n, π₁ p = ^#z ∧ π₂ p = ^#z) ∨
-      (∃ x, π₁ p = ^&x ∧ π₂ p = ^&(x + 1)) ∨
-      (∃ k f v v', π₁ p = ^func k f v ∧ π₂ p = ^func k f v' ∧ ∀ i u u', ⟪i, u⟫ ∈ v → ⟪i, u'⟫ ∈ v' → Shift L n ⟪u, u'⟫) ) :=
-  (construction L).case
-
-alias ⟨Shift.case, Shift.mk⟩ := Shift.case_iff
-
-lemma Shift.semiterm₁ {n t t'} (h : Shift L n ⟪t, t'⟫) : L.Semiterm n t := by simpa using h.case.1
-
-lemma Shift.semiterm₂ {n t t'} (h : Shift L n ⟪t, t'⟫) : L.Semiterm n t' := by simpa using h.case.2.1
-
-@[simp] lemma Shift.bvar {n z : V} (hz : z < n) :
-    Shift L n ⟪^#z, ^#z⟫ := Shift.mk ⟨by simp [hz], by simp [hz]⟩
-
-lemma Shift.bvar_iff {n z u : V} :
-    Shift L n ⟪^#z, u⟫ ↔ z < n ∧ u = ^#z :=
-  ⟨by intro h
-      rcases h.case with ⟨_, _, (⟨z', hz', hzz', h⟩ | ⟨x, h, _⟩ | ⟨k, f, v, v', h, _⟩)⟩
-      · rcases (show z = z' from by simpa using hzz'); exact ⟨hz', by simpa using h⟩
-      · simp [qqBvar, qqFvar] at h
-      · simp [qqBvar, qqFunc] at h,
-   by rintro ⟨hz, Hu, h⟩; exact Shift.bvar hz⟩
-
-@[simp] lemma Shift.fvar {n : V} (x : V):
-    Shift L n ⟪^&x, ^&(x + 1)⟫ := Shift.mk ⟨by simp, by simp⟩
-
-lemma Shift.fvar_iff {n x u : V} :
-    Shift L n ⟪^&x, u⟫ ↔ u = ^&(x + 1) :=
-  ⟨by intro h
-      rcases h.case with ⟨_, _, (⟨_, _, h, _⟩ | ⟨x', hx', h⟩ | ⟨_, _, _, _, h, _, _⟩)⟩
-      · simp [qqBvar, qqFvar] at h
-      · rcases (show x = x' by simpa using hx'); simpa using h
-      · simp [qqFvar, qqFunc] at h,
-   by rintro ⟨hz, Hu, h⟩; exact Shift.fvar x⟩
-
-lemma Shift.func {n k f v v' : V}
-    (hkf : L.Func k f)
-    (hv : L.TermSeq k n v)
-    (hv' : L.TermSeq k n v')
-    (H : ∀ i u u', ⟪i, u⟫ ∈ v → ⟪i, u'⟫ ∈ v' → Shift L n ⟪u, u'⟫) :
-    Shift L n ⟪^func k f v, ^func k f v'⟫ :=
-  Shift.mk ⟨
-    by rw [pi₁_pair]; exact Semiterm.func hkf hv,
-    by rw [pi₂_pair]; exact Semiterm.func hkf hv',
-    Or.inr <| Or.inr ⟨k, f, v, v', by simp, by simp, H⟩⟩
-
-lemma Shift.func' {n k f v u : V} (h : Shift L n ⟪^func k f v, u⟫) :
-    ∃ v', Seq v' ∧ k = lh v' ∧ (∀ i u u', ⟪i, u⟫ ∈ v → ⟪i, u'⟫ ∈ v' → Shift L n ⟪u, u'⟫) ∧ u = ^func k f v' := by
-  rcases h.case with ⟨_, hu, (⟨_, _, h, _⟩ | ⟨x, h, _⟩ | ⟨k', f', v', v'', h₁, h₂, hv⟩)⟩
-  · simp [qqFunc, qqBvar] at h
-  · simp [qqFunc, qqFvar] at h
-  · rcases (show k = k' ∧ f = f' ∧ v = v' by simpa [qqFunc] using h₁) with ⟨rfl, rfl, rfl⟩
-    rcases (show u = ^func k f v'' by simpa using h₂)
-    have : L.Func k f ∧ Seq v'' ∧ k = lh v'' ∧ ∀ i u, ⟪i, u⟫ ∈ v'' → L.Semiterm n u := by simpa [Semiterm.func_iff] using hu
-    rcases this with ⟨_, Sv'', hk'', _⟩
-    exact ⟨v'', Sv'', hk'', hv, rfl⟩
 
 variable {n : V}
 
-lemma Shift.rng_exists {t : V} (ht : L.Semiterm n t) : ∃ u, Shift L n ⟪t, u⟫ := by
-  apply Semiterm.induction 𝚺 ?_ ?_ ?_ ?_ t ht
-  · definability
-  · intro z hz; exact ⟨^#z, Shift.bvar hz⟩
-  · intro x; exact ⟨^&(x + 1), by simp⟩
-  · rintro k f v hkf hv ih
-    have : ∃ v', Seq v' ∧ lh v' = lh v ∧ ∀ i u', ⟪i, u'⟫ ∈ v' → ∀ u, ⟪i, u⟫ ∈ v → Shift L n ⟪u, u'⟫ := by
-      have : ∀ i < lh v, ∃ u', ∀ u, ⟪i, u⟫ ∈ v → Shift L n ⟪u, u'⟫ := by
-        intro i hi
-        have : ∃ u, Shift L n ⟪hv.seq.nth hi, u⟫ := ih i (hv.seq.nth hi) (by simp)
-        rcases this with ⟨u', hu'⟩
-        exact ⟨u', fun u hiuv  ↦ by rcases hv.seq.nth_uniq hi hiuv; exact hu'⟩
-      exact sigmaOne_skolem_seq
-        (by have : 𝚺₁-Relation fun x y ↦ ∀ u < v, ⟪x, u⟫ ∈ v → Shift L n ⟪u, y⟫ := by definability
-            exact this.of_iff fun w ↦ ⟨fun h u _ ↦ h u, fun h u hv ↦ h u (lt_of_mem_rng hv) hv⟩)
-        this
-    rcases this with ⟨v', Sv', hvv', h⟩
-    exact ⟨^func k f v',
-      Shift.func hkf hv ⟨Sv', by simp [hvv', hv.lh],
-        (fun i u' hi ↦ by
-          have : i < lh v := by simpa [hvv'] using Sv'.lt_lh_of_mem hi
-          exact h i u' hi (hv.seq.nth this) (by simp) |>.semiterm₂)⟩
-        (fun i u u' hi hi' ↦ h i u' hi' u hi)⟩
+@[simp] lemma termShift_bvar {z} (hz : z < n) :
+    L.termShift n #̂z = #̂z := by simp [Language.termShift, hz, construction]
 
-lemma Shift.rng_unique
-    {t u₁ u₂ : V} : Shift L n ⟪t, u₁⟫ → Shift L n ⟪t, u₂⟫ → u₁ = u₂ := by
-  revert u₁ u₂
-  suffices L.Semiterm n t → ∀ u₁ u₂, Shift L n ⟪t, u₁⟫ → Shift L n ⟪t, u₂⟫ → u₁ = u₂
-  by intro u₁ u₂ h₁ h₂; exact this h₁.semiterm₁ u₁ u₂ h₁ h₂
-  intro ht
-  apply Semiterm.induction 𝚷 ?_ ?_ ?_ ?_ t ht
-  · definability
-  · simp only [bvar_iff, and_imp]
-    rintro z _ u₁ u₂ _ rfl _ rfl; rfl
-  · simp [Shift.fvar_iff]
-  · intro k f v _ hv ih u₁ u₂ h₁ h₂
-    rcases Shift.func' h₁ with ⟨v₁, Sv₁, hk₁, hvv₁, rfl⟩
-    rcases Shift.func' h₂ with ⟨v₂, Sv₂, hk₂, hvv₂, rfl⟩
-    have : v₁ = v₂ := Sv₁.lh_ext Sv₂ (by simp [←hk₁, ←hk₂]) (by
-      intro i x₁ x₂ hxv₁ hxv₂
-      have hi : i < lh v := by simpa [←hv.lh, hk₁] using Sv₁.lt_lh_of_mem hxv₁
-      exact ih i (hv.seq.nth hi) (by simp) _ _ (hvv₁ _ _ _ (hv.seq.nth_mem hi) hxv₁) (hvv₂ _ _ _ (hv.seq.nth_mem hi) hxv₂))
-    rw [this]
+@[simp] lemma termShift_fvar (x) :
+    L.termShift n &̂x = &̂(x + 1) := by simp [Language.termShift, construction]
 
-lemma Shift.rng_exists_unique {t : V} (ht : L.Semiterm n t) : ∃! u, Shift L n ⟪t, u⟫ := by
-  rcases Shift.rng_exists ht with ⟨u, hu⟩
-  exact ExistsUnique.intro u hu (fun u' hu' ↦ Shift.rng_unique hu' hu)
-
-variable (L)
-
-lemma Shift.rng_exists_unique_total (n t : V) :
-    ∃! u, (L.Semiterm n t → Shift L n ⟪t, u⟫) ∧ (¬L.Semiterm n t → u = 0) := by
-  by_cases h : L.Semiterm n t
-  · simp [h]; exact Shift.rng_exists_unique h
-  · simp [h]
-
-end FormalizedTermShift
-
-open FormalizedTermShift
-
-variable (L)
-
-def Language.termShift (n t : V) : V := Classical.choose! (Shift.rng_exists_unique_total L n t)
-
-variable {L}
-
-lemma Language.Semiterm.termShift_spec {n t : V} (ht : L.Semiterm n t) : Shift L n ⟪t, L.termShift n t⟫ :=
-  Classical.choose!_spec (Shift.rng_exists_unique_total L n t) |>.1 ht
-
-lemma termShift_spec_of_not_termShift {n t : V} :
-    ¬L.Semiterm n t → L.termShift n t = 0 :=
-  Classical.choose!_spec (Shift.rng_exists_unique_total L n t) |>.2
-
-lemma Language.Semiterm.termShift_eq_of {n t} (ht : L.Semiterm n t) (h : Shift L n ⟪t, u⟫) : L.termShift n t = u :=
-  ht.termShift_spec.rng_unique h
-
-lemma termShift_bvar {z : V} (hz : z < n) : L.termShift n (^#z) = ^#z :=
-  Language.Semiterm.termShift_eq_of (by simp [hz]) (Shift.bvar hz)
-
-@[simp] lemma termShift_fvar (x : V) : L.termShift n (^&x) = ^&(x + 1) :=
-  Language.Semiterm.termShift_eq_of (by simp) (Shift.fvar x)
-
-lemma termShift_func {k f v v' : V} (hfk : L.Func k f)
-    (hv : L.TermSeq k n v)
-    (hv' : L.TermSeq k n v')
-    (H : ∀ i u u', ⟪i, u⟫ ∈ v → ⟪i, u'⟫ ∈ v' → L.termShift n u = u') : L.termShift n (^func k f v) = ^func k f v' :=
-  Language.Semiterm.termShift_eq_of (Semiterm.func hfk hv)
-    (Shift.func hfk hv hv' (fun i u u' hi hi' ↦ by
-      rcases H i u u' hi hi'
-      exact Language.Semiterm.termShift_spec (hv.prop i u hi)))
+@[simp] lemma termShift_func {k f v} (hkf : L.Func k f) (hv : L.SemitermSeq k n v) :
+    L.termShift n (f̂unc k f v) = f̂unc k f (L.termShiftSeq k n v) := by
+  simp [Language.termShift, construction, hkf, hv]; rfl
 
 section
 
+def _root_.LO.FirstOrder.Arith.LDef.termShiftDef (pL : LDef) : 𝚺₁-Semisentence 3 :=
+  (blueprint pL).result
+
+def _root_.LO.FirstOrder.Arith.LDef.termShiftSeqDef (pL : LDef) : 𝚺₁-Semisentence 4 := (blueprint pL).resultSeq
+
 variable (L)
 
-private lemma termShift_graph (u n t : V) :
-    u = L.termShift n t ↔
-    (L.Semiterm n t → ∃ p ≤ (t + u + 1)^2, p = ⟪t, u⟫ ∧ Shift L n p) ∧ (¬L.Semiterm n t → u = 0) :=
-  Iff.trans (Classical.choose!_eq_iff (Shift.rng_exists_unique_total L n t)) ⟨by
-    rintro ⟨hp, hn⟩
-    exact ⟨fun h ↦ ⟨⟪t, u⟫, by simp, rfl, hp h⟩, hn⟩, by
-    rintro ⟨hp, hn⟩
-    exact ⟨fun h ↦ by rcases hp h with ⟨_, _, rfl, h⟩; exact h, hn⟩⟩
-
-def _root_.LO.FirstOrder.Arith.LDef.termShiftDef (pL : LDef) : 𝚺₁-Semisentence 3 := .mkSigma
-  “u n t | (!pL.isSemitermDef.pi n t → ∃ p <⁺ (t + u + 1)², !pairDef p t u ∧ !(shiftDef pL).sigma n p) ∧ (¬!pL.isSemitermDef.sigma n t → u = 0)” (by simp)
-
 lemma termShift_defined : 𝚺₁-Function₂ L.termShift via pL.termShiftDef := by
-  intro v
-  simp [LDef.termShiftDef, termShift_graph, HSemiformula.val_sigma, eval_termSeq L,
-    eval_isSemitermDef L, (termSeq_defined L).proper.iff', (isSemiterm_defined L).proper.iff', eval_shiftDef L, -and_imp, -not_and]
+  intro v; simpa [LDef.termShiftDef, Language.termShift] using (construction L).result_defined v
 
-@[simp] lemma termShift_defined_iff (v : Fin 3 → V) :
+@[simp] lemma eval_termShiftDef (v : Fin 3 → V) :
     Semiformula.Evalbm (L := ℒₒᵣ) V v pL.termShiftDef ↔ v 0 = L.termShift (v 1) (v 2) := (termShift_defined L).df.iff v
 
 instance termShift_definable : 𝚺₁-Function₂ L.termShift :=
   Defined.to_definable _ (termShift_defined L)
 
+@[definability, simp] instance termShift_definable' (Γ i) : (Γ, i + 1)-Function₂ L.termShift := .of_sigmaOne (termShift_definable L) _ _
+
+lemma termShiftSeq_defined : 𝚺₁-Function₃ L.termShiftSeq via pL.termShiftSeqDef := by
+  intro v; simpa [LDef.termShiftSeqDef, Language.termShiftSeq] using (construction L).resultSeq_defined v
+
+@[simp] lemma eval_termShiftSeqDef (v : Fin 4 → V) :
+    Semiformula.Evalbm (L := ℒₒᵣ) V v pL.termShiftSeqDef ↔ v 0 = L.termShiftSeq (v 1) (v 2) (v 3) := (termShiftSeq_defined L).df.iff v
+
+instance termShiftSeq_definable : 𝚺₁-Function₃ L.termShiftSeq :=
+  Defined.to_definable _ (termShiftSeq_defined L)
+
+@[simp, definability] instance termShiftSeq_definable' (Γ i) : (Γ, i + 1)-Function₃ L.termShiftSeq :=
+  .of_sigmaOne (termShiftSeq_definable L) _ _
+
 end
 
+lemma termShift_rng_semiterm {t} (ht : L.Semiterm n t) : L.Semiterm n (L.termShift n t) := by
+  apply Language.Semiterm.induction 𝚺 ?_ ?_ ?_ ?_ t ht
+  · definability
+  · intro z hz; simp [hz]
+  · intro x; simp
+  · intro k f v hkf hv ih;
+    simp only [hkf, hv, termShift_func, Language.Semiterm.func_iff, true_and]
+    exact ⟨by simp [Language.termShiftSeq, hv], by simp [Language.termShiftSeq, hv], fun i z hiz ↦ by
+      rcases (construction L).resultSeq_prop' _ hv hiz with ⟨u, hiu, rfl⟩
+      exact ih _ _ hiu⟩
+
+lemma termShiftSeq_rng_termSeq {k n v} (hv : L.SemitermSeq k n v) : L.SemitermSeq k n (L.termShiftSeq k n v) :=
+  ⟨by simp [Language.termShiftSeq, hv], by simp [Language.termShiftSeq, hv], fun i u hiu ↦ by
+    rcases (construction L).resultSeq_prop' _ hv hiu with ⟨u', hiu', rfl⟩
+    exact termShift_rng_semiterm (hv.prop _ _ hiu')⟩
+
 end termShift
--/
+
+end
+
+namespace Formalized
+
+abbrev LOR : Arith.Language V := Language.codeIn ℒₒᵣ V
+
+notation "⌜ℒₒᵣ⌝" => LOR
+
+def zeroIndex : ℕ := Encodable.encode (Language.Zero.zero : (ℒₒᵣ : FirstOrder.Language).Func 0)
+
+def oneIndex : ℕ := Encodable.encode (Language.One.one : (ℒₒᵣ : FirstOrder.Language).Func 0)
+
+def addIndex : ℕ := Encodable.encode (Language.Add.add : (ℒₒᵣ : FirstOrder.Language).Func 2)
+
+def mulIndex : ℕ := Encodable.encode (Language.Mul.mul : (ℒₒᵣ : FirstOrder.Language).Func 2)
+
+def eqIndex : ℕ := Encodable.encode (Language.Eq.eq : (ℒₒᵣ : FirstOrder.Language).Rel 2)
+
+def ltIndex : ℕ := Encodable.encode (Language.LT.lt : (ℒₒᵣ : FirstOrder.Language).Rel 2)
+
+protected def zero : ℕ := f̂unc 0 zeroIndex ∅
+
+protected def one : ℕ := f̂unc 0 oneIndex ∅
+
+abbrev qqAdd (x y : V) := f̂unc 2 (addIndex : V) !⟦x, y⟧
+
+abbrev qqMul (x y : V) := f̂unc 2 (mulIndex : V) !⟦x, y⟧
+
+notation "𝟎" => Formalized.zero
+
+notation "𝟏" => Formalized.one
+
+infixl:60 " +̂  " => qqAdd
+
+infixl:80 " *̂ " => qqMul
+
+lemma qqFunc_absolute (k f v : ℕ) : ((f̂unc k f v : ℕ) : V) = f̂unc (k : V) (f : V) (v : V) := by simp [qqFunc, nat_cast_pair]
+
+@[simp] lemma LOR_func_zeroIndex : ⌜ℒₒᵣ⌝.Func 0 (zeroIndex : V) := by
+  simpa using codeIn_func_encode (M := V) (L := ℒₒᵣ) 0 Language.Zero.zero
+
+@[simp] lemma LOR_func_oneIndex : ⌜ℒₒᵣ⌝.Func 0 (oneIndex : V) := by
+  simpa using codeIn_func_encode (M := V) (L := ℒₒᵣ) 0 Language.One.one
+
+@[simp] lemma LOR_func_addIndex : ⌜ℒₒᵣ⌝.Func 2 (addIndex : V) := by
+  simpa using codeIn_func_encode (M := V) (L := ℒₒᵣ) 2 Language.Add.add
+
+@[simp] lemma LOR_func_mulIndex : ⌜ℒₒᵣ⌝.Func 2 (mulIndex : V) := by
+  simpa using codeIn_func_encode (M := V) (L := ℒₒᵣ) 2 Language.Mul.mul
+
+@[simp] lemma LOR_rel_eqIndex : ⌜ℒₒᵣ⌝.Rel 2 (eqIndex : V) := by
+  simpa using codeIn_rel_encode (M := V) (L := ℒₒᵣ) 2 Language.Eq.eq
+
+@[simp] lemma LOR_rel_ltIndex : ⌜ℒₒᵣ⌝.Rel 2 (ltIndex : V) := by
+  simpa using codeIn_rel_encode (M := V) (L := ℒₒᵣ) 2 Language.LT.lt
+
+@[simp] lemma zero_semiterm : ⌜ℒₒᵣ⌝.Semiterm n (𝟎 : V) := by
+  simp [Formalized.zero, qqFunc_absolute]
+
+@[simp] lemma one_semiterm : ⌜ℒₒᵣ⌝.Semiterm n (𝟏 : V) := by
+  simp [Formalized.one, qqFunc_absolute]
+
+namespace Numeral
+
+def blueprint : PR.Blueprint 0 where
+  zero := .mkSigma “y | y = !!(Semiterm.Operator.numeral ℒₒᵣ Formalized.one)” (by simp)
+  succ := .mkSigma “y t n | ∃ p,
+    !mkSeq₂Def p t !!(Semiterm.Operator.numeral ℒₒᵣ Formalized.one) ∧
+    !qqFuncDef y 2 !!(Semiterm.Operator.numeral ℒₒᵣ addIndex) p” (by simp)
+
+def construction : PR.Construction V blueprint where
+  zero := fun _ ↦ 𝟏
+  succ := fun _ _ t ↦ t +̂ 𝟏
+  zero_defined := by intro v; simp [blueprint, numeral_eq_natCast]
+  succ_defined := by intro v; simp [blueprint, numeral_eq_natCast]
+
+def numeralAux (x : V) : V := construction.result ![] x
+
+@[simp] lemma numeralAux_zero : numeralAux (0 : V) = 𝟏 := by simp [numeralAux, construction]
+
+@[simp] lemma numeralAux_succ (x : V) : numeralAux (x + 1) = numeralAux x +̂ 𝟏 := by simp [numeralAux, construction]
+
+section
+
+def numeralAuxDef : 𝚺₁-Semisentence 2 := blueprint.resultDef
+
+lemma numeralAux_defined : 𝚺₁-Function₁ (numeralAux : V → V) via numeralAuxDef :=
+  fun v ↦ by simp [construction.result_defined_iff, numeralAuxDef]; rfl
+
+@[simp] lemma eval_numeralAuxDef (v) :
+    Semiformula.Evalbm V v numeralAuxDef.val ↔ v 0 = numeralAux (v 1) := numeralAux_defined.df.iff v
+
+@[definability, simp] instance seqExp_definable : 𝚺₁-Function₁ (numeralAux : V → V) := Defined.to_definable _ numeralAux_defined
+
+end
+
+@[simp] lemma numeralAux_semiterm (n x : V) : ⌜ℒₒᵣ⌝.Semiterm n (numeralAux x) := by
+  induction x using induction_iSigmaOne
+  · definability
+  case zero => simp
+  case succ x ih => simp [ih]
+
+end Numeral
+
+section numeral
+
+open Numeral
+
+def numeral (x : V) : V := if x = 0 then 𝟎 else numeralAux (x - 1)
+
+@[simp] lemma numeral_zero : numeral (0 : V) = 𝟎 := by simp [numeral]
+
+@[simp] lemma numeral_semiterm (n x : V) : ⌜ℒₒᵣ⌝.Semiterm n (numeral x) := by
+  by_cases hx : x = 0 <;> simp [hx, numeral]
+
+section
+
+def numeralDef : 𝚺₁-Semisentence 2 := .mkSigma
+  “t x |
+    (x = 0 → t = !!(Semiterm.Operator.numeral ℒₒᵣ Formalized.zero)) ∧
+    (x ≠ 0 → ∃ x', !subDef x' x 1 ∧ !numeralAuxDef t x')”
+  (by simp)
+
+lemma numeral_defined : 𝚺₁-Function₁ (numeral : V → V) via numeralDef := fun v ↦ by
+  simp [numeralDef, numeral_eq_natCast]
+  by_cases hv1 : v 1 = 0 <;> simp [hv1, numeral]
+
+@[simp] lemma eval_numeralDef (v) :
+    Semiformula.Evalbm V v numeralDef.val ↔ v 0 = numeral (v 1) := numeral_defined.df.iff v
+
+@[definability, simp] instance numeral_definable : 𝚺₁-Function₁ (numeral : V → V) := Defined.to_definable _ numeral_defined
+
+@[definability, simp] instance numeral_definable' (Γ m) : (Γ, m + 1)-Function₁ (numeral : V → V) := .of_sigmaOne numeral_definable _ _
+
+end
+
+end numeral
+
+end Formalized
 
 end LO.Arith
 
